[wp definition] initial tests

theories/wp.v
@@ -1,4 +1,263 @@
 Require Import base lang free eval step safe.
 
-Definition wp η e φ :=
+From iris.proofmode Require Import base proofmode classes.
+
+From iris.base_logic.lib Require Import fancy_updates.
+From iris.bi Require Import weakestpre.
+From iris.prelude Require Import options.
+Import uPred.
+
+
+
+(* Keep the previous definition of [wp] based on [safe] for the examples using 
+ * it to remain valid. *)
+Definition old_wp η e φ :=
   safe (eval η e) φ.
+
+(* -------------------------------------------------------------------------- *)
+(* Definition of the meaning of being a value in [free val], as well as defining 
+ * a notion of stuckness. *)
+
+Definition to_val (m: free val) : option val :=
+  match m with
+  | Ret v => Some v
+  | _ => None
+  end.
+
+Lemma to_val_from_Ret (m: free val) (v: val) : to_val m = Some v -> m = Ret v.
+Proof.
+  unfold to_val.
+  by destruct m; inversion 1.
+Qed.
+
+Lemma to_val_non_Ret (m: free val) :
+  to_val m = None ->
+      m = Fail
+    ∨ m = free.Next
+    ∨ (∃ A B (c: code A B) x k, m = Stop c x k)
+    ∨ (∃ A1 A2 (m1: free A1) (m2: free A2) k (ko: unit → free val),
+        m = Par m1 m2 k ko).
+Proof.
+  destruct m; first inversion 1; intros?; eauto.
+  - do 2 right. left.
+    by eexists _, _, _, _, _.
+  - do 3 right.
+    by eexists _, _, _, _, _, _.
+Qed.
+
+(* Note: Per the lemma [only_fail_is_stuck], only fail is stuck.
+ * If this lemma remains (currently in discussion), it might be used to simplify 
+ * the definition below.
+ *)
+Definition not_stuck (m: free val): Prop :=
+  ~ stuck m.
+
+
+
+(* -------------------------------------------------------------------------- *)
+
+Class osirisGS_gen (hlc: has_lc) (Σ: gFunctor) := OsrisG {
+  osiris_invGS :> invGS_gen hlc Σ;
+
+  (* TODO: add the state interpretation *)
+}.
+
+
+
+(* -------------------------------------------------------------------------- *)
+(* Definition of the weakest precondition.
+ * This is heavily inspired from [iris/{bi,program_logic}/weakestpre.v].
+ *)
+
+(* TODO: push the modality towards [-∗] in the second branch. *)
+Definition wp_pre `{!osirisGS_gen hlc Σ} (s: stuckness)
+  (wp: coPset -d> free val -d> (val -d> iPropO Σ) -d> iPropO Σ):
+  coPset -d> free val -d> (val -d> iPropO Σ) -d> iPropO Σ :=
+  λ E m φ,
+    match to_val m with
+    | Some v => (|={E}=> φ v)%I
+    | None => (|={E}=> ⌜not_stuck m⌝
+        ∗ ∀ (m': free val),
+        ⌜step m m'⌝ -∗ ▷ wp E m' φ)%I
+    end.
+
+#[local]
+Instance wp_pre_contractive `{!osirisGS_gen hlc Σ} s : Contractive (wp_pre s).
+Proof.
+  rewrite /wp_pre /= => n wp wp' Hwp E m Φ.
+  repeat (f_contractive || f_equiv).
+  apply Hwp.
+Qed.
+
+(* Keeping the stuckness bit and the following notation ensure that the usual 
+ * notations will work (ie. [WP _ @ _ {{ _ }}] and [WP _@ _ ?{{ _ }}]). *)
+Definition wp_def `{!osirisGS_gen hlc Σ} : Wp (iProp Σ) (free val) val stuckness :=
+  λ (s: stuckness), fixpoint (wp_pre s).
+
+Local Definition wp_aux : seal (@wp_def). Proof. by eexists. Qed.
+Definition wp' := wp_aux.(unseal).
+Global Arguments wp' {hlc Σ _}.
+Global Existing Instance wp'.
+Local Lemma wp_unseal `{!osirisGS_gen hlc Σ} : wp = @wp_def hlc Σ _.
+Proof. rewrite -wp_aux.(seal_eq) //. Qed.
+
+
+
+(* -------------------------------------------------------------------------- *)
+(* Definitions and lemmas to better work with our WP.
+ * Once again, this is heavily inspired from 
+ * [iris/{bi,program_logic}/weakestpre.v] *)
+
+Section wp.
+  Context `{!osirisGS_gen hlc Σ}.
+  Implicit Types s : stuckness.
+  Implicit Types P : iProp Σ.
+  Implicit Types φ : val → iProp Σ.
+  Implicit Types v : val.
+  Implicit Types m : free val.
+
+  Lemma wp_unfold s E m φ :
+    WP m @ s; E {{ φ }} ⊣⊢ wp_pre s (wp (PROP:=iProp Σ) s) E m φ.
+  Proof.
+    rewrite wp_unseal.
+    (* TODO: remove φ which should not be necessary here. *)
+    apply (@fixpoint_unfold _ _ _ (wp_pre s) _ _ _ φ).
+  Qed.
+
+  Global Instance wp_ne s E m n :
+    Proper (pointwise_relation _ (dist n) ==> dist n) (wp (PROP:=iProp Σ) s E m).
+  Proof.
+    revert m. induction (lt_wf n) as [n _ IH]=> m Φ Ψ HΦ.
+    rewrite !wp_unfold /wp_pre /=.
+    (* Cf. the comment in [program_logic/wp.v] for an explanation on the time 
+     * taken by the following line. *)
+    do 7 (f_contractive || f_equiv).
+    rewrite IH; [done|lia|]. intros v. eapply dist_le; [apply HΦ|lia].
+  Qed.
+
+  Global Instance wp_proper s E m :
+    Proper (pointwise_relation _ (≡) ==> (≡)) (wp (PROP:=iProp Σ) s E m).
+  Proof.
+    by intros Φ Φ' ?; apply equiv_dist=>n; apply wp_ne=>v; apply equiv_dist.
+  Qed.
+  Global Instance wp_contractive s E m n :
+    TCEq (to_val m) None →
+    Proper (pointwise_relation _ (dist_later n) ==> dist n) (wp (PROP:=iProp Σ) s E m).
+  Proof.
+    intros He Φ Ψ HΦ. rewrite !wp_unfold /wp_pre He /=.
+    repeat (f_contractive || f_equiv).
+  Qed.
+
+
+
+  Lemma wp_value_fupd' s E Φ m v :
+    WP (Ret v) @ s; E {{ Φ }} ⊣⊢ |={E}=> Φ v.
+  Proof.
+    now rewrite wp_unfold /wp_pre /=.
+  Qed.
+
+  Lemma fupd_wp s E m (Φ: val -> iProp Σ) :
+    (|={E}=> WP m @ s; E {{ Φ }}) ⊢ WP m @ s; E {{ Φ }}.
+  Proof.
+    rewrite wp_unfold /wp_pre. iIntros "H". destruct (to_val m) as [v|] eqn:?.
+    { by iMod "H". }
+    iMod "H". iMod "H" as "[% H]".
+    iApply fupd_sep.
+    iSplitR.
+    { by iPureIntro. }
+    by iApply "H".
+  Qed.
+
+  Lemma wp_strong_mono s1 s2 E1 E2 m Φ Ψ :
+    s1 ⊑ s2 → E1 ⊆ E2 →
+    WP m @ s1; E1 {{ Φ }} -∗ (∀ v, Φ v ={E2}=∗ Ψ v) -∗ WP m @ s2; E2 {{ Ψ }}.
+  Proof.
+    iIntros (? HE) "H HΦ". iLöb as "IH" forall (m E1 E2 HE Φ Ψ).
+    rewrite !wp_unfold /wp_pre /=.
+    destruct (to_val m) as [v|] eqn:?.
+    { iApply ("HΦ" with "[> -]"). by iApply (fupd_mask_mono E1 _). }
+    iMod (fupd_mask_subseteq E1) as "Hclose"; first done.
+    iMod ("H") as "[% H]".
+    iMod "Hclose".
+    iModIntro. iSplit; [by destruct s1, s2|]. iIntros (m' Hstep).
+    iPoseProof ("H" $! m' Hstep) as "H".
+    iModIntro.
+    iApply ("IH" with "[//]H HΦ").
+  Qed.
+
+  Lemma wp_fupd s E m Φ : WP m @ s; E {{ v, |={E}=> Φ v }} ⊢ WP m @ s; E {{ Φ }}.
+  Proof.
+    iIntros "H".
+    iApply (wp_strong_mono s s E with "H"); auto.
+  Qed.
+
+End wp.
+
+
+
+(* -------------------------------------------------------------------------- *)
+(* The following are lemmas about the evolutions of a term. They are designed to 
+ * be used in [wp_tactics].
+ * Most of these lemmas have counterparts defined for [safe] in 
+ * [theories/safe.v]. (Note: as the step-indexing using [nat] is replaced by one 
+ * that uses the later modality, inductions are replaced by Löb inductions.)
+ *)
+
+Section wp_lemmas.
+  Context `{!osirisGS_gen hlc Σ}.
+  Implicit Types s : stuckness.
+  Implicit Types P : iProp Σ.
+  Implicit Types φ : val → iProp Σ.
+  Implicit Types v : val.
+  Implicit Types m : free val.
+
+  Lemma wp_ret s E v φ:
+    (|={E}=> φ v)
+    -∗ WP (Ret v) @ s; E {{ φ }}.
+  Proof. by rewrite!wp_unfold/wp_pre/=. Qed.
+
+  (* It might be useful to prove that there is no associate WP to [Fail] (should 
+   * be trivial because Fail is stuck (ie. not a value and does not reduce)). *)
+  Lemma wp_fail s E φ:
+    ⊢(WP Fail @ s; E {{ φ }}) -∗ ⌜False⌝.
+  Admitted.
+
+  (* To prove [WP (Par m1 m2 k ko) φ], one should provide two post conditions φ1 
+   * and φ2 and show that:
+   * - m1 satisfies the post-condition φ1
+   * - m2 satisfies the post-condition φ1
+   * - for any values v1 and v2 satisfying φ1 and φ2 respectively,
+   *     the pair (v1, v2) satisfies φ.
+  *)
+  Lemma wp_par s E m1 m2 k ko φ φ1 φ2:
+    WP m1 @ s ; E {{ φ1 }} -∗ WP m2 @ s ; E {{ φ2 }}
+    -∗ (∀ (v1 v2: val),
+        (φ1 v1) -∗ (φ2 v2)
+         -∗ WP (k (v1, v2)) @ s; E {{ φ }})
+      (*={E}=∗*) -∗ WP (Par m1 m2 k ko) @ s ; E {{ φ }}.
+  Proof.
+    iLöb as "IH".
+    iIntros "H1 H2 Hcomb".
+    rewrite !wp_unfold/wp_pre.
+    simpl.
+    destruct (to_val m1) as [v1|] eqn:E1;
+    destruct (to_val m2) as [v2|] eqn:E2.
+    { (* case [Par (Ret _) (Ret _) _ _] *)
+      apply to_val_from_Ret in E1 as ->, E2 as ->.
+      iApply fupd_sep.
+      iSplitR.
+      { iPureIntro. intros [_ H]. apply (H (k (v1, v2))), StepParRetRet. }
+      iPoseProof ("IH" with "[$H1][$H2][$Hcomb]") as "H".
+      iModIntro.
+      iIntros (m' Hstep).
+      destruct_step.
+      - admit.
+      - inversion Hstep.
+      - inversion Hstep. }
+  Admitted.
+End wp_lemmas.
+
+
+
+(* Keep a definition based on [safe] so that [examples.v] does not break. *)
+Definition wp := old_wp.
