theories/eval.v
@@ -1,4 +1,7 @@
 Require Import lang base free.
+Notation "x ← y ; z" := (bind y (λ x, z)).
+Notation "' x ← y ; z" := (bind y (λ x : _, z))
+  (at level 20, x pattern, y at level 100, z at level 200, only parsing) : stdpp_scope.
 
 (* Conventional metavariables. *)
 
